Fix module issue by creating Module Type
Create module type with int operations needed,
instantiate for Int and Int64
Now do not need to convert between sint and int,
types are equal

proofs/FEC/SeqCmp.v
@@ -1,6 +1,105 @@
 (*Comparing Sequence Numbers for an arbitrary wordsize*)
 Require Import VST.floyd.functional_base.
+
+(*We want sequence number comparison that works for both Int and Int64.
+  If we parameterize by the WORDSIZE directly, we end up with two
+  non-identical copies of Int/Int64 that we have to convert between.
+  Instead, we define a Module Type consisting only of the int
+  operations that we need for the sequence number comparison.
+  Then we instantiate this for both Int and Int64 (it could be
+    instantiated with any other size ints if needed).*)
+
+(*Problems if we have ssreflect in scope here*)
+Module Type IntType.
+
+Parameter wordsize: nat.
+Definition modulus : Z := two_power_nat wordsize.
+Definition half_modulus : Z := modulus / 2.
+Definition max_unsigned : Z := modulus - 1.
+Definition max_signed : Z := half_modulus - 1.
+Definition min_signed : Z := - half_modulus.
+
+Parameter int: Type.
+
+Parameter unsigned: int -> Z.
+Parameter signed: int -> Z.
+
+Parameter repr: Z -> int.
+Definition eq (x y: int) : bool :=
+  if zeq (unsigned x) (unsigned y) then true else false.
+Definition sub (x y: int) : int :=
+  repr (unsigned x - unsigned y).
+
+Axiom half_modulus_modulus: modulus = 2 * half_modulus.
+Axiom half_modulus_pos: half_modulus > 0.
+Axiom unsigned_repr_eq:
+  forall x, unsigned (repr x) = Z.modulo x modulus.
+Axiom signed_repr_eq:
+  forall x, signed (repr x) = if zlt (Z.modulo x modulus) half_modulus 
+  then Z.modulo x modulus else Z.modulo x modulus - modulus.
+
+Axiom eq_sym:
+forall x y, eq x y = eq y x.
+
+Axiom unsigned_range:
+  forall i, 0 <= unsigned i < modulus.
+Axiom signed_range:
+  forall i, min_signed <= signed i <= max_signed.
+
+End IntType.
+
+(*Instantiate for Int*)
+Module I32 <: IntType.
+
+Definition wordsize := Int.wordsize.
+Definition modulus := Int.modulus.
+Definition half_modulus := Int.half_modulus.
+Definition max_unsigned := Int.max_unsigned.
+Definition max_signed := Int.max_signed.
+Definition min_signed := Int.min_signed.
+Definition int := int.
+Definition unsigned := Int.unsigned.
+Definition signed := Int.signed.
+Definition repr := Int.repr.
+Definition eq := Int.eq.
+Definition sub := Int.sub.
+Definition half_modulus_modulus := Int.half_modulus_modulus.
+Definition half_modulus_pos := Int.half_modulus_pos.
+Definition unsigned_repr_eq := Int.unsigned_repr_eq.
+Definition signed_repr_eq := Int.signed_repr_eq.
+Definition eq_sym := Int.eq_sym.
+Definition unsigned_range := Int.unsigned_range.
+Definition signed_range := Int.signed_range.
+
+End I32.
+
+(*Instantiate for Int64*)
+Module I64 <: IntType.
+
+Definition wordsize := Int64.wordsize.
+Definition modulus := Int64.modulus.
+Definition half_modulus := Int64.half_modulus.
+Definition max_unsigned := Int64.max_unsigned.
+Definition max_signed := Int64.max_signed.
+Definition min_signed := Int64.min_signed.
+Definition int := Int64.int.
+Definition unsigned := Int64.unsigned.
+Definition signed := Int64.signed.
+Definition repr := Int64.repr.
+Definition eq := Int64.eq.
+Definition sub := Int64.sub.
+Definition half_modulus_modulus := Int64.half_modulus_modulus.
+Definition half_modulus_pos := Int64.half_modulus_pos.
+Definition unsigned_repr_eq := Int64.unsigned_repr_eq.
+Definition signed_repr_eq := Int64.signed_repr_eq.
+Definition eq_sym := Int64.eq_sym.
+Definition unsigned_range := Int64.unsigned_range.
+Definition signed_range := Int64.signed_range.
+
+End I64.
+
 From Coq Require Import ssreflect.
+
 
 Definition z_abs_diff (z1 z2: Z) : Z :=
   Z.abs (z1 - z2).
@@ -18,7 +117,7 @@ Proof.
   move=> z1 z2. rewrite /z_abs_diff. lia.
 Qed.
 
-Module SeqCmp(WS: WORDSIZE).
+Module SeqCmp (I: IntType).
 
 (*Integer comparison is more difficult - we don't want
   just Int.ltu - since 0 should be considered larger than
@@ -26,7 +125,7 @@ Module SeqCmp(WS: WORDSIZE).
   arithmetic" in RFC 1982 and the wikipedia article*)
   (*We use this for comparing times*)
 
-Module I := Make WS.
+(*Module I := Make WS.*)
 
 Ltac rep_lia_setup2 ::=
 pose_lemmas I.unsigned I.unsigned_range;
